%%%%%%%%%%%%%%%%%%%%%%%%%%%%%%%%%%%%%%%%%%%%%%%%%%%%%%%%%%%%%%%%%%%%%%
% CS624: Analysis of Algorithms
% Copyright 2015 Pejman Ghorbanzade <pejman@ghorbanzade.com>
% Creative Commons Attribution-ShareAlike 4.0 International License
% More info: https://github.com/ghorbanzade/beacon
%%%%%%%%%%%%%%%%%%%%%%%%%%%%%%%%%%%%%%%%%%%%%%%%%%%%%%%%%%%%%%%%%%%%%%

\section*{Question 6}

Prove that in a rooted tree $T$, if $x$ is an ancestor of $y$ and $y$ is an ancestor of $x$, then $x = y$.

\subsection*{Solution}

Proof is given by contradiction.
Assume $x$ is an ancestor of $y$ and $y$ is an ancestor of $x$ and $x \neq y$ ($x$ and $y$ are two distinct nodes).
According to definition of ancestorhood, there are paths from root $v_r$ of the form $v_r \rightarrow x \rightarrow y$ and $v_r \rightarrow y \rightarrow x$.
This immediately results to a simple loop of the form $x \rightarrow y \rightarrow x$ and $y \rightarrow x \rightarrow y$ which contradicts the definition of the tree.
Therefore the assumption is false and the proof is complete.
